common/theories/LoopChecking/Deciders.v
@@ -10,12 +10,6 @@ From Equations Require Import Equations.
 
 From MetaRocq.Common.LoopChecking Require Import Common Interfaces HornClauses Model Models PartialLoopChecking InitialSemilattice HornSemilatticeEquiv.
 
-Module Autorew.
-  Import Ltac2.
-  #[global] Ltac2 autorewrite0 ids cl :=
-  Std.autorewrite true None ids (default_on_concl cl).
-End Autorew.
-
 Set Equations Transparent.
 
 Module Type LoopCheckingItf (LS : LevelSets).
@@ -503,57 +497,6 @@ Proof.
     exists (y - z). now rewrite /min_atom_value (level_value_MapsTo hmap).
 Qed.
 
-Ltac lset :=
-  match goal with
-  | [ H : LevelSet.In _ (LevelSet.singleton _) |- _ ] =>
-    apply LevelSet.singleton_spec in H; red in H; try subst
-  | [ H : LevelSet.In _ (LevelSet.add _ _) |- _ ] =>
-    apply LevelSet.add_spec in H as []
-  | [ H : LevelSet.mem _ _ = false |- _ ] =>
-    apply LevelSetProp.FM.not_mem_iff in H
-  | [ H : LevelSet.mem _ _ = true |- _ ] =>
-    apply LevelSetProp.FM.mem_iff in H
-  | [ H : LevelExprSet.In _ (LevelExprSet.singleton _) |- _ ] =>
-    apply LevelExprSet.singleton_spec in H; red in H; try subst
-  | [ H : LevelExprSet.In _ (LevelExprSet.add _ _) |- _ ] =>
-    apply LevelExprSet.add_spec in H as []
-  | [ H : LevelMap.MapsTo _ _ (LevelMap.add _ _ _) |- _ ] =>
-    rewrite LevelMapFact.F.add_mapsto_iff in H; unfold Level.eq in H
-  | [ H : LevelMap.MapsTo _ _ (LevelMap.empty _) |- _ ] =>
-    rewrite LevelMapFact.F.empty_mapsto_iff in H; unfold Level.eq in H
-  | [ H : LevelSet.In _ (LevelSet.union _ _) |- _ ] =>
-    apply LevelSet.union_spec in H as []
-  | [ |- LevelSet.In _ (LevelSet.singleton _) ] =>
-    apply LevelSet.singleton_spec; rewrite ?/LevelSet.E.eq
-  | [ |- LevelSet.In _ (LevelSet.add _) ] =>
-    apply LevelSet.add_spec
-  | [ |- LevelSet.In _ (LevelSet.union _) ] =>
-    apply LevelSet.union_spec
-  | [ |- LevelSet.In _ (LevelSet.singleton _) -> _ ] =>
-    move/LevelSet.singleton_spec; rewrite ?/LevelSet.E.eq
-  | [ |- LevelSet.In _ (LevelSet.add _) -> _ ] =>
-    move/LevelSet.add_spec
-  | [ |- LevelSet.In _ (LevelSet.union _) -> _ ] =>
-    move/LevelSet.union_spec
-  end; try lsets.
-
-Hint Rewrite clauses_of_le_spec clauses_levels_spec
-  LevelSet.singleton_spec LevelSet.add_spec LevelSet.union_spec
-  LevelSetFact.is_empty_1 LevelSetFact.empty_iff
-  LevelExprSet.singleton_spec LevelExprSet.add_spec LevelExprSet.union_spec LevelExprSetFact.empty_iff
-  @NES.singleton_spec @NES.add_spec_les
-  Clauses.singleton_spec Clauses.add_spec Clauses.union_spec ClausesFact.empty_iff
-  LevelMapFact.F.add_mapsto_iff LevelMapFact.F.empty_mapsto_iff
-  : set_specs.
-
-Hint Rewrite <- LevelSetProp.FM.not_mem_iff LevelSetProp.FM.mem_iff : set_specs.
-
-Ltac rsets := repeat (progress (autorewrite with set_specs || lset || intro
-  || unfold Level.eq, LevelSet.E.eq in * )).
-
-Ltac2 Notation "rsets" cl(opt(clause)) :=
-  let id := Option.get (Ident.of_string "set_specs") in
-  Autorew.autorewrite0 [id] cl.
 
 Definition init_clause_of_level l :=
   (singleton (l, 0), (Level.zero, if Level.is_global l then 1 else 0)).
@@ -783,6 +726,41 @@ Module CorrectModel.
 
   Definition clauses_sem {S} {SL : Semilattice S Q.t} (V : Level.t -> S) (cls : Clauses.t) : Prop :=
     Clauses.For_all (clause_sem V) cls.
+
+  Instance clauses_sem_proper {S} {SL : Semilattice S Q.t} :
+    Proper (Logic.eq ==> Clauses.Equal ==> iff) clauses_sem.
+  Proof.
+    move=> ?? -> ?? h.
+    rewrite /clauses_sem.
+    now rewrite h.
+  Qed.
+
+  Lemma clauses_sem_singleton {S} {SL : Semilattice S Q.t} {V cl} :
+    clauses_sem V (Clauses.singleton cl) <-> clause_sem V cl.
+  Proof.
+    rewrite /clauses_sem /Clauses.For_all.
+    split; firstorder. apply H. clsets.
+    apply Clauses.singleton_spec in H0. now subst.
+  Qed.
+
+  Lemma clauses_sem_add {S} {SL : Semilattice S Q.t} {V cl cls} :
+    clauses_sem V (Clauses.add cl cls) <-> clause_sem V cl /\ clauses_sem V cls.
+  Proof.
+    rewrite /clauses_sem /Clauses.For_all.
+    split.
+    - intros hcl. split.
+      * apply hcl, Clauses.add_spec; now left.
+      * move=> x hin; apply hcl, Clauses.add_spec; now right.
+    - move=> [] hcl hcls x /Clauses.add_spec -[]. now subst.
+      apply hcls.
+  Qed.
+
+  Lemma clauses_sem_union {S} {SL : Semilattice S Q.t} {V cls cls'} :
+    clauses_sem V (Clauses.union cls cls') <-> clauses_sem V cls /\ clauses_sem V cls'.
+  Proof.
+    rewrite /clauses_sem /Clauses.For_all.
+    setoid_rewrite Clauses.union_spec. firstorder.
+  Qed.
 
 
   Definition to_val (v : LevelMap.t nat) l :=
@@ -1250,18 +1228,7 @@ Module Abstract.
       exists x. firstorder. now rsets.
   Qed.
   Hint Rewrite @clauses_levels_add : set_specs.
-
-  Lemma levelexprset_singleton {l le} : (exists k : Z, LevelExprSet.In (l, k) (singleton le)) <-> (l, le.2) = le.
-  Proof.
-    split.
-    - move=> [] k. rsets. now subst le.
-    - intros <-. exists le.2; now rsets.
-  Qed.
   Hint Rewrite @levelexprset_singleton : set_specs.
-
-  Lemma levels_singleton le : NES.levels (LevelExprSet.singleton le) =_lset LevelSet.singleton le.1.
-  Proof. intros l; rewrite NES.levels_spec. rsets. split; intros h; subst. destruct h. rsets. exists le.2.
-    rsets. now destruct le. Qed.
   Hint Rewrite levels_singleton : set_specs.
 
   Lemma clause_levels_init_constraint l : clause_levels (init_clause_of_level l)
@@ -1529,41 +1496,6 @@ Module Abstract.
         exists k. split => //. now apply LevelExprSet.add_spec.
   Qed.
 
-  Instance clauses_sem_proper {S} {SL : Semilattice S Q.t} :
-    Proper (Logic.eq ==> Clauses.Equal ==> iff) clauses_sem.
-  Proof.
-    move=> ?? -> ?? h.
-    rewrite /clauses_sem.
-    now rewrite h.
-  Qed.
-
-  Lemma clauses_sem_singleton {S} {SL : Semilattice S Q.t} {V cl} :
-    clauses_sem V (Clauses.singleton cl) <-> clause_sem V cl.
-  Proof.
-    rewrite /clauses_sem /Clauses.For_all.
-    split; firstorder. apply H. clsets.
-    apply Clauses.singleton_spec in H0. now subst.
-  Qed.
-
-  Lemma clauses_sem_add {S} {SL : Semilattice S Q.t} {V cl cls} :
-    clauses_sem V (Clauses.add cl cls) <-> clause_sem V cl /\ clauses_sem V cls.
-  Proof.
-    rewrite /clauses_sem /Clauses.For_all.
-    split.
-    - intros hcl. split.
-      * apply hcl, Clauses.add_spec; now left.
-      * move=> x hin; apply hcl, Clauses.add_spec; now right.
-    - move=> [] hcl hcls x /Clauses.add_spec -[]. now subst.
-      apply hcls.
-  Qed.
-
-  Lemma clauses_sem_union {S} {SL : Semilattice S Q.t} {V cls cls'} :
-    clauses_sem V (Clauses.union cls cls') <-> clauses_sem V cls /\ clauses_sem V cls'.
-  Proof.
-    rewrite /clauses_sem /Clauses.For_all.
-    setoid_rewrite Clauses.union_spec. firstorder.
-  Qed.
-
   Lemma clauses_sem_leq {S} {SL : Semilattice S Q.t} (V : Level.t -> S) l r :
     clauses_sem V (l ⋞ r) <->
     (interp_prems V l ≤ interp_prems V r)%sl.
@@ -1802,6 +1734,18 @@ Module LoopChecking (LS : LevelSets).
     check m c <-> valid_entailments (clauses m) (to_clauses c).
   Proof. apply check_clauses_complete. Qed.
 
+  Lemma check_declared m c :
+    check m c -> LevelSet.Subset (clauses_levels (to_clauses c)) (levels m).
+  Proof.
+    rewrite /check /Impl.check_clauses.
+    move: (to_clauses c) => cls.
+    move/Clauses.for_all_spec.
+    move: cls; apply: ClausesProp.set_induction.
+    - intros s he.
+     cl. hin.
+
+
+
   (* Returns the valuation of the model: a minimal assignement from levels to constraints
     that make the enforced clauses valid. *)
   Definition valuation m := to_val (Model.valuation_of_model (model m)).
@@ -1820,5 +1764,14 @@ Module LoopChecking (LS : LevelSets).
 
   Lemma above_zero_declared m : Impl.CorrectModel.above_zero_declared (levels m) (clauses m).
   Proof. eapply above_zero_declared. Qed.
+
+  Lemma model_valuation_zero m : valuation m Level.zero = 0%nat.
+  Proof. apply valuation_0. Qed.
+
+  Lemma model_valuation_global {m l} : LevelSet.In l (levels m) -> Level.is_global l -> (valuation m l > 0)%nat.
+  Proof. apply valuation_global. Qed.
+
+  Lemma model_valuation_not_global {m l} : LevelSet.In l (levels m) -> ~~ Level.is_global l -> (valuation m l >= 0)%nat.
+  Proof. apply valuation_not_global. Qed.
 
 End LoopChecking.
